Merge simplification and OCaml splitting.

src/covering.ml
@@ -42,7 +42,6 @@ open Evd
 open Evarutil
 open Evar_kinds
 open Equations_common
-open Depelim
 open Termops
 open Syntax
 
@@ -213,8 +212,8 @@ let typecheck_map env evars (ctx, subst, ctx') =
       ctx' subst []
   in ()
 
-let check_ctx_map env evars map =
-  if debug then
+let check_ctx_map ?(unsafe = false) env evars map =
+  if debug && not unsafe then
     try typecheck_map env evars map; map
     with Type_errors.TypeError (env, e) ->
       errorlabstrm "equations"
@@ -230,8 +229,8 @@ let check_ctx_map env evars map =
 	   spc () ++ str"Anomaly: " ++ CErrors.print e)
   else map
     
-let mk_ctx_map env evars ctx subst ctx' =
-  let map = (ctx, subst, ctx') in check_ctx_map env evars map
+let mk_ctx_map ?(unsafe = false) env evars ctx subst ctx' =
+  let map = (ctx, subst, ctx') in check_ctx_map ~unsafe env evars map
 
 let rec map_patterns f ps =
   List.map (function
@@ -322,8 +321,57 @@ and lift_patns n k = map (lift_patn n k)
 let lift_pat n p = lift_patn n 0 p
 let lift_pats n p = lift_patns n 0 p
 
+let make_permutation ?(env = Global.env ()) (sigma : Evd.evar_map)
+  ((ctx1, pats1, _) : context_map) ((ctx2, pats2, _) : context_map) : context_map =
+    let len = List.length ctx1 in
+    let perm = Array.make len None in
+    let merge_rels i1 i2 =
+        match perm.(pred i2) with
+        | None -> perm.(pred i2) <- Some i1
+        | Some j when Int.equal i1 j -> ()
+        | _ -> failwith "Could not generate a permutation"
+    in
+    let rec collect_rels k acc c =
+      if Term.isRel c then
+        let x = Term.destRel c in
+        if k < x && x <= len + k then x - k :: acc
+        else acc
+      else Termops.fold_constr_with_binders succ collect_rels k acc c
+    in
+    let merge_constrs c1 c2 =
+      let rels1 = collect_rels 0 [] c1 in
+      let rels2 = collect_rels 0 [] c2 in
+      try List.iter2 merge_rels rels1 rels2
+      with Invalid_argument _ -> failwith "Could not generate a permutation"
+    in
+    (* FIXME This function could also check that constructors are the same and
+     * so on. It also need better error handling. *)
+    let env1 = Environ.push_rel_context ctx1 env in
+    let env2 = Environ.push_rel_context ctx2 env in
+    let merge_pats pat1 pat2 =
+      let c1 = constr_of_pat env1 pat1 in
+      let c2 = constr_of_pat env2 pat2 in
+      let c1 = Tacred.compute env1 sigma c1 in
+      let c2 = Tacred.compute env2 sigma c2 in
+        merge_constrs c1 c2
+    in
+    List.iter2 merge_pats pats1 pats2;
+    let pats = Array.map (function
+                          | None -> failwith "Could not generate a permutation"
+                          | Some i -> PRel i) perm in
+    let pats = Array.to_list pats in
+      mk_ctx_map env sigma ctx1 pats ctx2
+
 type unification_result = 
   (context_map * int * constr * pat) option
+
+let rec context_map_of_splitting : splitting -> context_map = function
+  | Compute (subst, _, _, _) -> subst
+  | Split (subst, _, _, _) -> subst
+  | Valid (subst, _, _, _, _, _) -> subst
+  | Mapping (subst, _) -> subst
+  | RecValid (_, s) -> context_map_of_splitting s
+  | Refined (subst, _, _) -> subst
 
 let specialize_mapping_constr (m : context_map) c = 
   specialize_constr (pi2 m) c
@@ -442,6 +490,70 @@ let strengthen ?(full=true) ?(abstract=false) env evd (ctx : rel_context) x (t :
   in
     (ctx', subst, ctx), reorder
 
+(* TODO Merge both strengthening functions. Bottom one might be better. *)
+(* Return a substitution (and its inverse) which is just a permutation
+ * of the variables in the context which is well-typed, and such that
+ * all variables in [t] (and their own dependencies) are now declared
+ * before [x] in the context. *)
+let new_strengthen (env : Environ.env) (evd : Evd.evar_map) (ctx : Context.Rel.t)
+  (x : int) ?(rels : Int.Set.t = rels_above ctx x) (t : Term.constr) :
+    context_map * context_map =
+  let rels = Int.Set.union rels (dependencies_of_term env evd ctx t x) in
+  let maybe_reduce k t =
+    if Int.Set.mem k (Termops.free_rels t) then
+      Equations_common.nf_betadeltaiota env evd t
+    else t
+  in
+  (* We may have to normalize some declarations in the context if they
+   * mention [x] syntactically when they shouldn't. *)
+  let ctx = CList.map_i (fun k decl ->
+    if Int.Set.mem k rels && k < x then
+      Equations_common.map_rel_declaration (maybe_reduce (x - k)) decl
+    else decl) 1 ctx in
+  (* Now we want to put everything in [rels] as the oldest part of the context,
+   * and everything else after. The invariant is that the context
+   * [subst (rev (before @ after)) @ ctx] is well-typed. *)
+  (* We also create along what we need to build the actual substitution. *)
+  let len_ctx = Context.Rel.length ctx in
+  let lifting = len_ctx - Int.Set.cardinal rels in
+  let rev_subst = Array.make len_ctx (PRel 0) in
+  let rec aux k before after n subst = function
+  | decl :: ctx ->
+      if Int.Set.mem k rels then
+        let subst = PRel (k + lifting - n + 1) :: subst in
+        rev_subst.(k + lifting - n) <- PRel k;
+        (* We lift the declaration not to be well-typed in the new context,
+         * but so that it reflects in a raw way its movement in the context.
+         * This allows to apply a simple substitution afterwards, instead
+         * of going through the whole context at each step. *)
+        let decl = Equations_common.map_rel_declaration (Vars.lift (n - lifting - 1)) decl in
+        aux (succ k) (decl :: before) after n subst ctx
+      else
+        let subst = PRel n :: subst in
+        rev_subst.(n - 1) <- PRel k;
+        let decl = Equations_common.map_rel_declaration (Vars.lift (k - n)) decl in
+        aux (succ k) before (decl :: after) (succ n) subst ctx
+  | [] -> CList.rev (before @ after), CList.rev subst
+  in
+  (* Now [subst] is a list of indices which represents the substitution
+   * that we must apply. *)
+  (* Right now, [ctx'] is an ill-typed rel_context, we need to apply [subst]. *)
+  let (ctx', subst) = aux 1 [] [] 1 [] ctx in
+  let rev_subst = Array.to_list rev_subst in
+  (* Fix the context [ctx'] by using [subst]. *)
+  (* We lift each declaration to make it appear as if it was under the
+   * whole context, which allows then to apply the substitution, and lift
+   * it back to its place. *)
+  let do_subst k c = Vars.lift (-k)
+    (specialize_constr subst (Vars.lift k c)) in
+  let ctx' = CList.map_i (fun k decl ->
+    Equations_common.map_rel_declaration (do_subst k) decl) 1 ctx' in
+  (* Now we have everything need to build the two substitutions. *)
+  let s = mk_ctx_map env evd ctx' subst ctx in
+  let rev_s = mk_ctx_map env evd ctx rev_subst ctx' in
+    s, rev_s
+
+
 let id_pats g = rev (patvars_of_tele g)
 let id_subst g = (g, id_pats g, g)
 	
@@ -469,9 +581,9 @@ let check_eq_context_nolet env sigma (_, _, g as snd) (d, _, _ as fst) =
     (str "Contexts do not agree for composition: "
        ++ pr_context_map env snd ++ str " and " ++ pr_context_map env fst)
 
-let compose_subst env ?(sigma=Evd.empty) ((g',p',d') as snd) ((g,p,d) as fst) =
-  if debug then check_eq_context_nolet env sigma snd fst;
-  mk_ctx_map env sigma g' (specialize_pats p' p) d
+let compose_subst ?(unsafe = false) env ?(sigma=Evd.empty) ((g',p',d') as snd) ((g,p,d) as fst) =
+  if debug && not unsafe then check_eq_context_nolet env sigma snd fst;
+  mk_ctx_map ~unsafe env sigma g' (specialize_pats p' p) d
 (*     (g', (specialize_pats p' p), d) *)
 
 let push_mapping_context decl (g,p,d) =
@@ -495,7 +607,7 @@ let lift_subst env evd (ctx : context_map) (g : rel_context) =
   let map = List.fold_right (fun decl acc -> push_mapping_context decl acc) g ctx in
     check_ctx_map env evd map
     
-let single_subst env evd x p g =
+let single_subst ?(unsafe = false) env evd x p g =
   let t = pat_constr p in
     if eq_constr t (mkRel x) then
       id_subst g
@@ -511,7 +623,7 @@ let single_subst env evd x p g =
       (* let pats = list_tabulate  *)
       (* 	(fun i -> let k = succ i in if k = x then p else PRel k) *)
       (* 	(List.length g) *)
-      in mk_ctx_map env evd substctx pats g
+      in mk_ctx_map ~unsafe env evd substctx pats g
     else
       let (ctx, s, g), _ = strengthen env evd g x t in
       let x' = match nth s (pred x) with PRel i -> i | _ -> error "Occurs check singleton subst"
@@ -520,7 +632,7 @@ let single_subst env evd x p g =
 	   in the context and the patterns. *)
       let substctx = subst_in_ctx x' t' ctx in
       let pats = List.map_i (fun i p -> subst_constr_pat x' (lift (-1) t') p) 1 s in
-	mk_ctx_map env evd substctx pats g
+	mk_ctx_map ~unsafe env evd substctx pats g
     
 exception Conflict
 exception Stuck
@@ -1265,6 +1377,14 @@ let rec covering_aux env evars data prev clauses path (ctx,pats,ctx' as prob) le
 			   mkRel var) sortinv
 		in args, !argref
 	      in
+              (* Don't forget section variables. *)
+              let secvars =
+                let named_context = Environ.named_context env in
+                  List.map (fun decl ->
+                    let id = Context.Named.Declaration.get_id decl in
+                    Constr.mkVar id) named_context
+              in
+              let secvars = Array.of_list secvars in
 	      let evar = new_untyped_evar () in
 	      let path' = evar :: path in
 	      let lets' =
@@ -1283,7 +1403,7 @@ let rec covering_aux env evars data prev clauses path (ctx,pats,ctx' as prob) le
 		      refined_arg = refarg;
 		      refined_path = path';
 		      refined_ex = evar;
-		      refined_app = (mkEvar (evar, [||]), strength_app);
+		      refined_app = (mkEvar (evar, secvars), strength_app);
 		      refined_revctx = revctx;
 		      refined_newprob = newprob;
 		      refined_newprob_to_lhs = newprob_to_lhs;
