src/splitting.ml
@@ -190,7 +190,93 @@ let term_of_tree status isevar env0 tree =
 	  Proofview.return pv', 
 	  it_mkLambda_or_LetIn (subst_vars substc c) ctx, it_mkProd_or_LetIn ty ctx
 	      
-    | Split ((ctx, _, _), rel, ty, sp) -> 
+    | Split ((ctx, _, _) as subst, rel, ty, sp) ->
+      if !Equations_common.ocaml_splitting then
+        (* Produce parts of a case that will be relevant. *)
+        let evd = ref evm in
+        let ctx', case_ty, branches_res, nb_cuts, rev_subst, to_apply, simpl =
+          Sigma_types.smart_case env evd ctx rel ty in
+
+        (* The next step is to use [simplify]. *)
+        let simpl_step = if simpl then
+          Simplify.simplify [Loc.dummy_loc, Simplify.Infer_many] env evd
+          else Simplify.identity env evd
+        in
+        let branches = Array.map2 (fun (ty, nb, csubst) next ->
+          (* We get the context from the constructor arity. *)
+          let new_ctx, ty = Term.decompose_prod_n_assum nb ty in
+          let new_ctx = Namegen.name_context env new_ctx in
+          let ty =
+            if simpl || nb_cuts > 0 then
+              let env = Environ.push_rel_context (new_ctx @ ctx') env in
+              Tacred.hnf_constr env !evd ty
+            else ty
+          in
+          (* Remove the cuts and append them to the context. *)
+          let cut_ctx, ty = Term.decompose_prod_n_assum nb_cuts ty in
+
+          (* TODO This context should be the same as (pi1 csubst). We could
+           * either optimize (but names in [csubst] are worse) or just insert
+           * a sanity-check. *)
+          (*
+          let () =
+            let ctx = cut_ctx @ new_ctx @ ctx' in
+            msg_info(str"Simplifying term:");
+            msg_info(let env = Environ.push_rel_context ctx env in
+              Printer.pr_constr_env env !evd ty);
+            msg_info(str"... in context:");
+            msg_info(Printer.pr_rel_context env !evd ctx)
+          in
+          *)
+          let ((hole, c), lsubst) = simpl_step (cut_ctx @ new_ctx @ ctx', ty) in
+          let subst = Covering.compose_subst ~unsafe:true env ~sigma:!evd csubst subst in
+          let subst = Covering.compose_subst ~unsafe:true env ~sigma:!evd lsubst subst in
+          (* Now we build a term to put in the match branch. *)
+          let c =
+            match hole, next with
+            (* Dead code: we should have found a proof of False. *)
+            | None, None -> c
+            (* Normal case: build recursively a subterm. *)
+            | Some ((next_ctx, _), ev), Some s ->
+                let evm, next_term, next_ty = aux env !evd s in
+                (* Now we need to instantiate [ev] with the term [next_term]. *)
+                let conv_fun = Evarconv.evar_conv_x Names.full_transparent_state in
+                let next_env = Environ.push_rel_context next_ctx env in
+                (* [next_term] starts with lambdas, so we apply it to its context. *)
+                let args = Equations_common.extended_rel_vect 0 next_ctx in
+                let next_term = Reduction.beta_appvect next_term args in
+                (* Finally, we might need to permutate some rels. *)
+                let next_subst = Covering.context_map_of_splitting s in
+                let perm_subst = Covering.make_permutation evm subst next_subst in
+                let next_term = Covering.mapping_constr perm_subst next_term in
+                evd := Evarsolve.evar_define conv_fun next_env evm None ev next_term;
+                c
+            (* This should not happen... *)
+            | _ -> failwith "Should not fail here, please report."
+          in
+            Term.it_mkLambda_or_LetIn c (cut_ctx @ new_ctx)
+        ) branches_res sp in
+
+        (* Get back to the original context. *)
+        let case_ty = Covering.mapping_constr rev_subst case_ty in
+        let branches = Array.map (Covering.mapping_constr rev_subst) branches in
+
+        (* Fetch the type of the variable that we want to eliminate. *)
+        let after, decl, before = Covering.split_context (pred rel) ctx in
+        let rel_ty = Context.Rel.Declaration.get_type decl in
+        let rel_ty = Vars.lift rel rel_ty in
+        let rel_t = Constr.mkRel rel in
+        let pind, _ = Inductive.find_inductive env rel_ty in
+
+        (* Build the case. *)
+        let case_info = Inductiveops.make_case_info env (fst pind) Constr.RegularStyle in
+        let case = Constr.mkCase (case_info, case_ty, rel_t, branches) in
+        let term = Constr.mkApp (case, Array.of_list to_apply) in
+        let term = Term.it_mkLambda_or_LetIn term ctx in
+        let typ = it_mkProd_or_subst ty ctx in
+        Typing.e_check env evd term typ;
+          !evd, term, typ
+      else
 	let before, decl, after = split_tele (pred rel) ctx in
 	let evd = ref evm in
 	let branches = 
