src/syntax.ml
@@ -50,7 +50,6 @@ open Evd
 open Evarutil
 open Evar_kinds
 open Equations_common
-open Depelim
 
 open Constrintern
 open Decl_kinds
