theories/DepElimDec.v
@@ -11,6 +11,37 @@ From Equations Require Import Init Signature DepElim EqDec.
 (** Alternative implementation of generalization using sigma types only,
    allowing to use K on decidable domains. *)
 
+(* Use the new simplification. *)
+(* FIXME Temporary location? *)
+Ltac simplify_one_dep_elim' :=
+match goal with
+(* Do not put any part of the rhs in the hypotheses. *)
+| |- let _ := block in _ => fail 1
+| |- _ => simplify ?
+(* Fallback for JMeq. *)
+| |- @JMeq _ _ _ _ -> _ => refine (@simplification_heq _ _ _ _ _)
+(* Trying with more primitive tactics. *)
+| |- ?f ?x = ?g ?y -> _ => let H := fresh in progress (intros H ; injection H ; clear H)
+| |- Id (?f ?x) (?g ?y) -> _ => let H := fresh in progress (intros H ; inversion H ; clear H)
+| |- ?t = ?u -> _ => let hyp := fresh in
+  intros hyp ; elimtype False ; discriminate
+| |- Id ?t ?u -> _ => let hyp := fresh in
+  intros hyp ; elimtype False ; solve [inversion hyp]
+| |- ?x = ?y -> _ => let hyp := fresh in
+  intros hyp ; (try (clear hyp ; (* If non dependent, don't clear it! *) fail 1)) ;
+    case hyp
+| |- Id _ ?x ?y -> _ => let hyp := fresh in
+  intros hyp ; (try (clear hyp ; (* If non dependent, don't clear it! *) fail 1)) ;
+    case hyp
+| |- _ -> ?B => let ty := type of B in (* Works only with non-dependent products *)
+  intro || (let H := fresh in intro H)
+| |- forall x, _ =>
+  let H := fresh x in intro H
+| |- _ => intro
+end.
+
+Ltac simplify_dep_elim ::= repeat simplify_one_dep_elim'.
+
 (** Decompose existential packages. *)
 
 (* Definition sigT_elim {A} {P : A -> Type} {P0 : sigma _ P -> Type} : *)
